Add a helper for extracting symmetry relations
Add sym_rel_with_same_key (with a SetUnfoldElemOf instance) to relate
events that share the same customised key. The helper then is used
to define loc, sthd, and val.

Add [SetUnfoldElemOf] instances

Add more [SetUnfoldElemOf] instances

Add [EID.t] to the filter of [collect_all]

Fix naming

Make [collect_all] take a predicate

Address comments and refactor

Tweak

Clean up and formatting

Revert removal of [val]

Formatting

Renaming

GenModels/CandidateExecutions.v
@@ -26,7 +26,10 @@ Require Import TermModels.
 Open Scope Z_scope.
 Open Scope stdpp_scope.
 
-Module CandidateExecutions (IWD : InterfaceWithDeps) (Term : TermModelsT IWD). (* to be imported *)
+
+
+(* to be imported *)
+Module CandidateExecutions (IWD : InterfaceWithDeps) (Term : TermModelsT IWD).
   Import IWD.
   Import Term.
   Notation outcome := (IWD.outcome DepOn.t empOutcome).
@@ -61,6 +64,11 @@ Module CandidateExecutions (IWD : InterfaceWithDeps) (Term : TermModelsT IWD). (
       sauto.
     Qed.
   End EID.
+
+
+  (* Add a hint for resolving decision instances *)
+  #[export] Hint Extern 10 (Decision (match ?x with _ => _ end)) =>
+    destruct x : typeclass_instances.
 
   Module Candidate.
 
@@ -187,151 +195,149 @@ Module CandidateExecutions (IWD : InterfaceWithDeps) (Term : TermModelsT IWD). (
 
     (*** Accessors ***)
 
-    Definition collect_all (P : iEvent -> bool) (cd : t) : gset EID.t :=
-      filter (fun '(eid, event) => P event) (event_list cd)
+    Definition collect_all (P : EID.t -> iEvent -> Prop)
+      `{∀ eid event, Decision (P eid event)}
+      (cd : t) : gset EID.t :=
+      filter (fun '(eid, event) => P eid event) (event_list cd)
         |> map fst |> list_to_set.
-
-    Global Instance set_elem_of_collect_all eid P cd :
-      SetUnfoldElemOf eid (collect_all P cd) (∃x, cd !! eid = Some x ∧ P x).
+    Global Instance set_elem_of_collect_all eid P
+      `{∀ eid event, Decision (P eid event)} cd :
+      SetUnfoldElemOf eid (collect_all P cd) (∃x, cd !! eid = Some x ∧ P eid x).
     Proof. tcclean. set_unfold. hauto db:pair. Qed.
     Global Typeclasses Opaque collect_all.
 
     (** Get the set of all valid EID for that candidate *)
-    Definition valid_eid (cd : t) :=
-      collect_all (fun event => true) cd.
+    Definition valid_eids (cd : t) :=
+      collect_all (fun _ _ => true) cd.
 
+    Global Instance set_elem_of_valid_eids eid cd :
+      SetUnfoldElemOf eid (valid_eids cd) (∃ x, cd !! eid = Some x).
+    Proof. tcclean. set_unfold. hauto db:pair. Qed.
+    Global Typeclasses Opaque valid_eids.
+
+    Definition is_reg_read (event : iEvent) : Prop :=
+      match event with
+      | IEvent (RegRead _ _) _ => true
+      | _ => false
+      end.
+
+    Global Instance is_reg_read_decision event : (Decision (is_reg_read event)).
+    Proof. unfold is_reg_read. apply _. Qed.
 
     (** Get the set of all register reads *)
     Definition reg_reads (cd : t) :=
-      collect_all
-        (fun event =>
-           match event with
-           | IEvent (RegRead _ _) _ => true
-           | _ => false end)
-        cd.
+      collect_all (λ _ event, is_reg_read event) cd.
 
-    Global Instance set_elem_of_reg_read eid cd :
-      SetUnfoldElemOf eid (reg_reads cd)
-        (∃ reg reg_acc res,
-            cd !! eid = Some (IEvent (RegRead reg reg_acc) res)).
-    Proof. tcclean. set_unfold. hauto l:on. Qed.
-    Global Typeclasses Opaque reg_reads.
+    Definition is_reg_write (event : iEvent) : Prop :=
+      match event with
+      | IEvent (RegWrite _ _ _ _) _ => true
+      | _ => false
+      end.
+
+    Global Instance is_reg_write_decision event : (Decision (is_reg_write event)).
+    Proof. unfold is_reg_write. apply _. Qed.
 
     (** Get the set of all register writes *)
     Definition reg_writes (cd : t) :=
-      collect_all
-        (fun event =>
-           match event with
-           | IEvent (RegWrite _ _ _ _) _ => true
-           | _ => false end)
-        cd.
+      collect_all (λ _ event, is_reg_write event) cd.
 
-    Global Instance set_elem_of_reg_writes eid cd :
-      SetUnfoldElemOf eid (reg_writes cd)
-        (∃ reg reg_acc dep val,
-            cd !! eid = Some (IEvent (RegWrite reg reg_acc dep val) ())).
-    Proof. tcclean. set_unfold. sauto dep:on. Qed.
-    Global Typeclasses Opaque reg_writes.
+    Definition is_mem_read (event : iEvent) : Prop :=
+      match event with
+      | IEvent (MemRead _ _) _ => true
+      | _ => false
+      end.
+
+    Global Instance is_mem_read_decision event : (Decision (is_mem_read event)).
+    Proof. unfold is_mem_read. apply _. Qed.
 
     (** Get the set of all memory reads *)
     Definition mem_reads (cd : t) :=
-      collect_all
-        (fun event =>
-           match event with
-           | IEvent (MemRead _ _) _ => true
-           | _ => false end)
-        cd.
+      collect_all (λ _ event, is_mem_read event) cd.
 
-    Global Instance set_elem_of_mem_reads eid cd :
-      SetUnfoldElemOf eid (mem_reads cd)
-        (∃ n rr res, cd !! eid = Some (IEvent (MemRead n rr) res)).
-    Proof. tcclean. set_unfold. hauto l:on. Qed.
-    Global Typeclasses Opaque mem_reads.
+    Definition is_mem_write (event : iEvent) :=
+      match event with
+      | IEvent (MemWrite _ _) _ => true
+      | _ => false
+      end.
+
+    Global Instance is_mem_write_decision event : (Decision (is_mem_write event)).
+    Proof. unfold is_mem_write. apply _. Qed.
 
     (** Get the set of all memory writes *)
     Definition mem_writes (cd : t) :=
-      collect_all
-        (fun event =>
-           match event with
-           | IEvent (MemWrite _ _) _ => true
-           | _ => false end)
-        cd.
+      collect_all (λ _ event, is_mem_write event) cd.
 
-    Global Instance set_elem_of_mem_writes eid cd :
-      SetUnfoldElemOf eid (mem_writes cd)
-        (∃ n wr res, cd !! eid = Some (IEvent (MemWrite n wr) res)).
-    Proof. tcclean. set_unfold. hauto l:on. Qed.
-    Global Typeclasses Opaque mem_writes.
+    Definition is_mem_event (event : iEvent) : Prop :=
+      match event with
+      | IEvent (MemRead _ _) _ => true
+      | IEvent (MemWrite _ _) _ => true
+      | _ => false
+      end.
+
+    Global Instance is_mem_event_decision event : (Decision (is_mem_event event)).
+    Proof. unfold is_mem_event. apply _. Qed.
 
     (** Get the set of all memory writes *)
     Definition mem_events (cd : t) :=
-      collect_all
-        (fun event =>
-           match event with
-           | IEvent (MemRead _ _) _ => true
-           | IEvent (MemWrite _ _) _ => true
-           | _ => false end)
-        cd.
+      collect_all (λ _ event, is_mem_event event) cd.
 
-    (** Get the set of all barriers *)
+    Definition is_branch (event : iEvent) : Prop :=
+      match event with
+      | IEvent (BranchAnnounce _ _) _ => true
+      | _ => false
+      end.
+
+    Global Instance is_branch_decision event : (Decision (is_branch event)).
+    Proof. unfold is_branch. apply _. Qed.
+
+    (** Get the set of all branches *)
     Definition branches (cd : t) :=
-      collect_all
-        (fun event =>
-           match event with
-           | IEvent (BranchAnnounce _ _) _ => true
-           | _ => false end)
-        cd.
-
-    (** Get the set of all barriers *)
-    Definition barriers (cd : t) :=
-      collect_all
-        (fun event =>
-           match event with
-           | IEvent (Barrier _) _ => true
-           | _ => false end)
-        cd.
+      collect_all (λ _ event, is_branch event) cd.
 
     (** Get the content of a barrier, returns none if not a barrier (or is an
         invalid EID) *)
-    Definition get_barrier (cd : t) (eid : EID.t) : option barrier:=
-      match cd !! eid with
-      | Some (IEvent (Barrier b) ()) => Some b
+    Definition get_barrier (event : iEvent) : option barrier:=
+      match event with
+      | IEvent (Barrier b) () => Some b
+      | _ => None
+      end.
+
+    (** Get the set of all barriers *)
+    Definition barriers (cd : t) :=
+      collect_all (λ _ event, is_Some (get_barrier event)) cd.
+
+    (** Get the content of a TLB operation, returns none if not a TLB operation
+        (or is an invalid EID) *)
+    Definition get_tlbop (event : iEvent) : option tlb_op :=
+      match event with
+      | IEvent (TlbOp _ to) () => Some to
       | _ => None
       end.
 
     (** Get the set of all TLB operations *)
-    Definition tlbops (cd : t) :=
-      collect_all
-        (fun event =>
-           match event with
-           | IEvent (TlbOp _ _) _ => true
-           | _ => false end)
-        cd.
-
-    (** Get the content of a TLB operation, returns none if not a TLB operation
-        (or is an invalid EID) *)
-    Definition get_tlbop (cd : t) (eid : EID.t) : option tlb_op :=
-      match cd !! eid with
-      | Some (IEvent (TlbOp _ to) ()) => Some to
-      | _ => None
-      end.
+    Definition tlpops (cd : t) :=
+      collect_all (λ _ event, is_Some (get_tlbop event)) cd.
 
     (*** Utility relations ***)
 
     (** Intra instruction order *)
     Definition iio (cd : t) := po cd ∩ si cd.
 
+    (** NOTE: make the dependencies opaque, and directly define wellformedness
+        conditions for them for now *)
     Definition addr (cd : t) :=
       ⦗mem_reads cd⦘⨾
         (⦗mem_reads cd⦘ ∪ (iio_data cd ⨾ (rrf cd ∪ ⦗reg_writes cd⦘))⁺)⨾
         iio_addr cd⨾
         ⦗mem_events cd⦘.
+    Global Typeclasses Opaque addr.
 
     Definition data (cd : t) :=
       ⦗mem_reads cd⦘⨾
         (⦗mem_reads cd⦘ ∪ (iio_data cd ⨾ (rrf cd ∪ ⦗reg_writes cd⦘))⁺)⨾
         iio_data cd⨾
         ⦗mem_events cd⦘.
+    Global Typeclasses Opaque data.
 
     Definition ctrl (cd : t) :=
       ⦗mem_reads cd⦘⨾
@@ -339,23 +345,198 @@ Module CandidateExecutions (IWD : InterfaceWithDeps) (Term : TermModelsT IWD). (
         iio_ctrl cd⨾
         ⦗branches cd⦘⨾
         (po cd ∖ si cd).
+    Global Typeclasses Opaque ctrl.
+
+
+    Definition gather_by_key_aux `{Countable K} (cd : t) (b : gmap K (gset EID.t))
+      (P : EID.t -> iEvent -> option K) :=
+      fold_left (λ acc '(eid, event), (match (P eid event) with
+                                       | Some k => {[ k := {[eid]}]}
+                                       | None =>  ∅
+                                       end) ∪ₘ acc) (event_list cd) b.
+
+    (** This helper computes an optional key from each eid and event pair of a
+        candidate using [get_key], and gathers all eids with the same key
+        together into a set. It returns a map from keys to sets of eids *)
+    Definition gather_by_key `{Countable K} (cd : t)
+      (get_key : EID.t -> iEvent -> option K) :=
+      gather_by_key_aux cd (∅ : gmap K (gset EID.t)) get_key.
+
+    Lemma lookup_total_unfold_gather_by_key_aux `{Countable K} (cd : t)
+      (get_key : EID.t -> iEvent -> option K) (b : gmap K (gset EID.t)) (k: K):
+      (forall k, b !!! k ## collect_all (λ _ _, true) cd) ->
+      gather_by_key_aux cd b get_key !!! k =
+      (b !!! k ∪ collect_all (λ eid event, (get_key eid event) =? Some k) cd).
+    Proof.
+      unfold gather_by_key_aux, valid_eids, collect_all. revert b.
+      pose proof (event_list_NoDup1 cd) as Hdup.
+
+      induction (event_list cd); first set_solver.
+      assert (map fst (filter (λ '(_, _), True) l) = l.*1) as Heql.
+      { clear. induction l; first done.
+        rewrite filter_cons_True. hauto lq:on use: map_cons. hauto. }
+
+      destruct a as [eid event].
+      rewrite fmap_cons in Hdup. specialize (IHl (NoDup_cons_1_2 _ _ Hdup)).
+      apply NoDup_cons_1_1 in Hdup.
+      do 2 rewrite filter_cons; simpl.
+
+      intros b Hb;simpl. rewrite IHl.
+      - destruct (get_key eid event);
+          (case_decide as Hk;[rewrite bool_unfold in Hk; inversion Hk; subst|]).
+        + rewrite lookup_total_unfold; set_solver + Hb.
+        + assert (k ≠ k0) as Hnk by naive_solver.
+          rewrite lookup_total_unfold; set_solver + Hb.
+        + rewrite lookup_total_unfold; set_solver +.
+      - intros k'. case_match eqn:PP.
+        + destruct (decide (k0 = k')).
+          * subst k0. rewrite lookup_total_unfold.
+            rewrite Heql. rewrite Heql in Hb. set_solver + Hb Hdup.
+          * rewrite lookup_total_unfold; set_solver + Hb.
+        + rewrite lookup_total_unfold; set_solver + Hb.
+    Qed.
+
+    (** The set of eids with key [k] in the gathered map generated with [get_key]
+        is equiv to the set of all eids filtered with [get_key] *)
+    Lemma lookup_total_unfold_gather_by_key `{Countable K} (cd : t)
+      (get_key : EID.t -> iEvent -> option K) (k: K):
+      gather_by_key cd get_key !!! k =
+      collect_all (λ eid event, (get_key eid event) =? Some k) cd.
+    Proof.
+      rewrite lookup_total_unfold_gather_by_key_aux.
+      rewrite lookup_total_empty. set_solver +.
+      intros. rewrite lookup_total_empty. set_solver +.
+    Qed.
+
+    Global Instance set_elem_of_gather_by_key_lookup `{Countable K} (cd : t)
+      (get_key : EID.t -> iEvent -> option K) (k: K) (eid : EID.t):
+      SetUnfoldElemOf eid (gather_by_key cd get_key !!! k)
+        (∃ E, cd !! eid = Some E ∧ get_key eid E = Some k).
+    Proof.
+      tcclean. rewrite lookup_total_unfold_gather_by_key. set_unfold.
+      split; intros [? Heq]. rewrite bool_unfold in Heq. all:hauto.
+    Qed.
+
+    Lemma lookup_is_Some_gather_by_key_aux `{Countable K} (cd : t)
+      (get_key : EID.t -> iEvent -> option K) (k: K) b:
+      (is_Some (b !! k) ∨ ∃ eid event, (eid, event) ∈ event_list cd
+                                       ∧ get_key eid event = Some k) ->
+       is_Some((gather_by_key_aux cd b get_key) !! k).
+    Proof.
+      unfold gather_by_key_aux. revert b.
+      induction (event_list cd); intros ? Hinit; first set_solver.
+      simpl. destruct a as [eid event]. destruct Hinit as [Hinit|Hinit].
+      apply IHl. destruct Hinit. left. case_match. destruct (decide (k = k0)).
+      subst k0. exists ({[eid]} ∪ x).
+      assert (Some {[eid]} ∪ₒ Some x = Some ({[eid]} ∪ x)) as <-. done.
+      apply lookup_unfold_pointwise_union. tcclean.
+      rewrite lookup_singleton_Some; hauto. done.
+     + exists x. assert (None ∪ₒ Some x = Some x) as <-. done.
+       apply lookup_unfold_pointwise_union. tcclean.
+       rewrite lookup_singleton_None; hauto. done.
+     + exists x. assert (None ∪ₒ Some x = Some x) as <-. done.
+       apply lookup_unfold_pointwise_union. tcclean.
+       rewrite lookup_empty; hauto. done.
+     + destruct Hinit as (?&?&Hcons&HP).
+       rewrite elem_of_cons in Hcons. destruct Hcons as [Hhd | Hin].
+       inversion Hhd; subst.
+       * rewrite HP. apply IHl. left.
+         destruct (b !! k) eqn:Hb.
+         exists ({[eid]} ∪ g).
+         assert (Some {[eid]} ∪ₒ Some g = Some ({[eid]} ∪ g)) as <-. done.
+         apply lookup_unfold_pointwise_union. tcclean.
+         rewrite lookup_singleton_Some; hauto. done.
+         exists {[eid]}. assert (Some {[eid]} ∪ₒ None = Some {[eid]}) as <-. done.
+         apply lookup_unfold_pointwise_union. tcclean.
+         rewrite lookup_singleton_Some; hauto. done.
+       * apply IHl. right. do 2 eexists. naive_solver.
+    Qed.
+
+    (** if exists an event with key [k], them [k] must in the gathered map *)
+    Lemma lookup_is_Some_gather_by_key `{Countable K} (cd : t)
+      (get_key : EID.t -> iEvent -> option K) (k: K):
+      (∃ eid event, (eid, event) ∈ event_list cd ∧ get_key eid event = Some k) ->
+       is_Some((gather_by_key cd get_key) !! k).
+    Proof.
+      unfold gather_by_key. intro Hexists.
+      apply lookup_is_Some_gather_by_key_aux. right; hauto.
+    Qed.
+
+    (** returns a symmetric relation, such that two events in the relation have
+        the same key computed with [get_key] *)
+    Definition sym_rel_with_same_key `{Countable K} (cd : t)
+      (get_key : EID.t -> iEvent -> option K) :=
+      let map : gmap K (gset EID.t) :=
+        gather_by_key cd get_key in
+      map_fold (fun (k : K) (s : gset EID.t) (r : grel EID.t) => r ∪ (s × s))
+        ∅ map.
+
+    (** A local unfold instance for [map_fold] with an union combinator which is
+        used in [sym_rel_by_key] *)
+    Local Instance set_elem_of_map_fold_set_union `{Countable K, Countable K'}
+      {V} (m : gmap K V) b e (f : K -> V -> gset K') :
+      SetUnfoldElemOf (e)
+        (map_fold (fun (k: K) (v : V) (r : gset K') => r ∪ (f k v)) b m)
+        (e ∈ b ∨ ∃ k v, m !! k = Some v ∧ e ∈ (f k v)).
+    Proof.
+      tcclean. cinduction m using map_fold_cind.
+      hauto lq:on use:lookup_empty_Some.
+      set_unfold. setoid_rewrite H2; clear H2.
+      split.
+      - intros [[| (?&?&?&?)]|]; first hauto lq:on;
+          (destruct (decide (e ∈ b)); [hauto lq:on | right; do 2 eexists;
+                                                     rewrite lookup_insert_Some;
+                                                     sauto lq:on]).
+      - intros [|(?&?&Hlk&?)]; first hauto lq:on;
+          rewrite lookup_insert_Some in Hlk; hauto lq:on.
+    Qed.
+
+    (** An unfold instance for [sym_rel_by_key] *)
+    Global Instance set_elem_of_sym_rel_with_same_key `{Countable K} cd
+      get_key eid1 eid2 :
+      SetUnfoldElemOf (eid1, eid2)
+        (sym_rel_with_same_key cd get_key)
+        (∃ E1 E2 (k: K), cd !! eid1 = Some E1 ∧ cd !! eid2 = Some E2
+                         ∧ get_key eid1 E1 = Some k ∧ get_key eid2 E2 = Some k).
+    Proof.
+      tcclean. set_unfold.
+      split.
+      - intros [|(k&?&Hfold&?)]; first done.
+        pose proof (lookup_total_unfold_gather_by_key cd get_key k) as Hunfold.
+        rewrite lookup_total_alt in Hunfold. rewrite Hfold in Hunfold. set_unfold.
+        pose proof (Hunfold eid1) as [(E1 & Hlk1 & Heq1) _]; first set_solver.
+        pose proof (Hunfold eid2) as [(E2 & Hlk2 & Heq2) _]; first set_solver.
+        repeat rewrite bool_unfold in *.
+        hauto lq:on.
+      - intros (?&?&k&Hlk1&Hloc1&?&Hloc2); right.
+        feed pose proof (lookup_is_Some_gather_by_key cd get_key k) as HSome.
+        set_unfold. hauto.
+        destruct HSome as [? HSome].
+        pose proof (lookup_total_unfold_gather_by_key cd get_key k) as Hunfold.
+        rewrite lookup_total_alt in Hunfold.
+        rewrite HSome in Hunfold. simpl in Hunfold.
+        do 2 eexists. split.
+        + eassumption.
+        + set_unfold. do 2 rewrite Hunfold.
+          split;eexists;(split;[eassumption|rewrite bool_unfold;hauto lq:on]).
+    Qed.
+
+    (** get physical address of an event *)
+    Definition get_pa (e : iEvent) : option (Arch.pa):=
+      match e with
+      | IEvent (MemRead _ rr) _ => Some (rr.(ReadReq.pa))
+      | IEvent (MemWrite n rr) _ => Some (rr.(WriteReq.pa))
+      | _ => None
+      end.
 
     (** Symmetry relation referring to events having the same address.
         Might need to be updated for mixed-size *)
     Definition loc (cd : t) : grel EID.t :=
-      let pa_map : gmap pa (gset EID.t) :=
-        fold_left
-        (fun pa_map '(eid, event) =>
-           match event : iEvent with
-           | IEvent (MemRead _ rr) _ => {[rr.(ReadReq.pa):= {[eid]}]} ∪ₘ pa_map
-           | IEvent (MemWrite n rr) _ => {[rr.(WriteReq.pa):= {[eid]}]} ∪ₘ pa_map
-           | _ => pa_map
-           end) (event_list cd) ∅ in
-      map_fold (fun (k : pa) (s : gset EID.t) (r : grel EID.t) => r ∪ (s × s))
-        ∅ pa_map.
+      sym_rel_with_same_key cd (λ _ event, get_pa event).
 
-
-
+    (** Symmetry relation referring to events of a same thread *)
+    Definition sthd (cd : t) : grel EID.t :=
+      sym_rel_with_same_key cd (λ eid _, Some (eid.(EID.tid))).
 
   End Candidate.
 
@@ -363,42 +544,20 @@ Module CandidateExecutions (IWD : InterfaceWithDeps) (Term : TermModelsT IWD). (
   Module NMSWF.
     Import Candidate.
 
+    (** Get 8 bytes values*)
+    Definition get_val (event : iEvent) :=
+      match event : iEvent with
+      | IEvent (MemRead 8 rr) (inl (val, _)) =>
+          Some val
+      | IEvent (MemWrite 8 rr) _ =>
+          Some (rr.(WriteReq.value))
+      | _ => None
+      end.
+
     (** This relation only make sense for 8-bytes non-mixed-size models.
         It relates events with the same values *)
     Definition val (cd : t) : grel EID.t :=
-      let val_map : gmap (bv 64) (gset EID.t) :=
-        fold_left
-        (fun val_map '(eid, event) =>
-           match event : iEvent with
-           | IEvent (MemRead 8 rr) (inl (val, _)) =>
-               {[val := {[eid]}]} ∪ₘ val_map
-           | IEvent (MemWrite 8 rr) _ =>
-               {[rr.(WriteReq.value) := {[eid]}]} ∪ₘ val_map
-           | _ => val_map
-           end) (event_list cd) ∅ in
-      map_fold (fun (k : bv 64) (s : gset EID.t) (r : grel EID.t) => r ∪ (s × s))
-        ∅ val_map.
-
-    Definition tlbops (cd : t) :=
-      collect_all
-        (fun event =>
-           match event with
-           | IEvent (TlbOp _ _) _ => true
-           | _ => false end)
-        cd.
-
-    (** Check that all memory accesses have size 8. Alignment checking need to
-        know how pa work and thus need to be architecture specific*)
-    Definition size8_wf (cd : t) : bool :=
-      collect_all
-        (fun event =>
-           match event with
-           | IEvent (MemRead 8 _) _ => false
-           | IEvent (MemRead _ _) _ => true
-           | IEvent (MemWrite 8 _) _ => false
-           | IEvent (MemWrite _ _) _ => true
-           | _ => false
-           end) cd =? ∅.
+      sym_rel_with_same_key cd (λ _ event, get_val event).
 
     Definition co_wf (cd : t) : bool :=
       let co := co cd in
